<?xml version="1.0"?>
<rdf:RDF xmlns="http://seodwarf.eu/ontology/v1.0#"
     xml:base="http://seodwarf.eu/ontology/v1.0"
     xmlns:swe="https://sweet.jpl.nasa.gov/sweet2.3/"
     xmlns:owl="http://www.w3.org/2002/07/owl#"
     xmlns:gn="http://www.geonames.org/ontology"
     xmlns:xsd="http://www.w3.org/2001/XMLSchema#"
     xmlns:rdfs="http://www.w3.org/2000/01/rdf-schema#"
     xmlns:dbo="http://dbpedia.org/resource/"
     xmlns:geo="http://www.eionet.europa.eu/gemet"
     xmlns:dct="http://dublincore.org/documents/2012/06/14/dcmiterms/"
     xmlns:rdf="http://www.w3.org/1999/02/22-rdf-syntax-ns#"
     xmlns:xml="http://www.w3.org/XML/1998/namespace"
     xmlns:strdf="http://strdf.di.uoa.gr/ontology/"
     xmlns:seo="http://seodwarf.eu/ontology/v1.0">
    <owl:Ontology rdf:about="http://seodwarf.eu/ontology/v1.0">
        <owl:versionIRI rdf:resource="http://seodwarf.eu/ontology/v1.0/1.0.0"/>
        <rdfs:label>SEO-DWARF Environment Ontology</rdfs:label>
    </owl:Ontology>
    


    <!-- 
    ///////////////////////////////////////////////////////////////////////////////////////
    //
    // Object Properties
    //
    ///////////////////////////////////////////////////////////////////////////////////////
     -->

    


    <!-- http://seodwarf.eu/ontology/v1.0#hasPhenomenon -->

    <owl:ObjectProperty rdf:about="http://seodwarf.eu/ontology/v1.0#hasPhenomenon">
        <rdf:type rdf:resource="http://www.w3.org/2002/07/owl#FunctionalProperty"/>
        <rdfs:domain rdf:resource="http://seodwarf.eu/ontology/v1.0#SatelliteImage"/>
        <rdfs:range rdf:resource="http://seodwarf.eu/ontology/v1.0#Phenomenon"/>
        <rdfs:comment>It describes the phenomenon present in the region of
reference. It refers to the “image_SEO-DWARF_phenomenon” concept. It is
defined as the “Part” property of the Dublin Core Ontology</rdfs:comment>
        <rdfs:isDefinedBy>dct:hasPart</rdfs:isDefinedBy>
    </owl:ObjectProperty>
    


    <!-- 
    ///////////////////////////////////////////////////////////////////////////////////////
    //
    // Data properties
    //
    ///////////////////////////////////////////////////////////////////////////////////////
     -->

    


    <!-- http://seodwarf.eu/ontology/v1.0#hasAbstract -->

    <owl:DatatypeProperty rdf:about="http://seodwarf.eu/ontology/v1.0#hasAbstract">
        <rdfs:domain rdf:resource="http://seodwarf.eu/ontology/v1.0#SatelliteImage"/>
        <rdfs:range rdf:resource="http://www.w3.org/2001/XMLSchema#string"/>
        <rdfs:comment>It describes the presence of a text description of the image. It
accepts alphanumerical values and it is defined as “abstract” property of the Dublin
Core Ontology</rdfs:comment>
        <rdfs:isDefinedBy>dct:abstract</rdfs:isDefinedBy>
    </owl:DatatypeProperty>
    


    <!-- http://seodwarf.eu/ontology/v1.0#hasBoundingBox -->

    <owl:DatatypeProperty rdf:about="http://seodwarf.eu/ontology/v1.0#hasBoundingBox">
        <rdfs:domain rdf:resource="http://seodwarf.eu/ontology/v1.0#SatelliteImage"/>
        <rdfs:range rdf:resource="http://www.w3.org/2001/XMLSchema#string"/>
        <rdfs:comment>Represents the Bounding Box of the Image in WKT</rdfs:comment>
    </owl:DatatypeProperty>
    


    <!-- http://seodwarf.eu/ontology/v1.0#hasClass -->

    <owl:DatatypeProperty rdf:about="http://seodwarf.eu/ontology/v1.0#hasClass">
        <rdfs:domain rdf:resource="http://seodwarf.eu/ontology/v1.0#Phenomenon"/>
        <rdfs:range rdf:resource="http://www.w3.org/2001/XMLSchema#string"/>
        <rdfs:comment>Represents the class for the phenomenon</rdfs:comment>
    </owl:DatatypeProperty>
    


    <!-- http://seodwarf.eu/ontology/v1.0#hasFormat -->

    <owl:DatatypeProperty rdf:about="http://seodwarf.eu/ontology/v1.0#hasFormat">
        <rdfs:domain rdf:resource="http://seodwarf.eu/ontology/v1.0#SatelliteImage"/>
        <rdfs:range rdf:resource="http://www.w3.org/2001/XMLSchema#string"/>
        <rdfs:comment>It describes the format of the image (raster or raw). It accepts
alphanumerical values</rdfs:comment>
    </owl:DatatypeProperty>
    


    <!-- http://seodwarf.eu/ontology/v1.0#hasIdentifier -->

    <owl:DatatypeProperty rdf:about="http://seodwarf.eu/ontology/v1.0#hasIdentifier">
        <rdf:type rdf:resource="http://www.w3.org/2002/07/owl#FunctionalProperty"/>
        <rdfs:domain rdf:resource="http://seodwarf.eu/ontology/v1.0#SatelliteImage"/>
        <rdfs:range rdf:resource="http://www.w3.org/2001/XMLSchema#string"/>
        <rdfs:comment>It describes presence of a unique identifier of the image in the
project. It accepts alphanumerical values and it is defined as the “identifier”
property of the Dublin Core Ontology.</rdfs:comment>
        <rdfs:isDefinedBy>dct:identifier</rdfs:isDefinedBy>
    </owl:DatatypeProperty>
    


    <!-- http://seodwarf.eu/ontology/v1.0#hasLineage -->

    <owl:DatatypeProperty rdf:about="http://seodwarf.eu/ontology/v1.0#hasLineage">
        <rdfs:domain rdf:resource="http://seodwarf.eu/ontology/v1.0#SatelliteImage"/>
        <rdfs:range rdf:resource="http://www.w3.org/2001/XMLSchema#string"/>
        <rdfs:comment>It is a field containing different textual information about the image.
The content depends by the operator that fills it. It accepts alphanumerical values</rdfs:comment>
    </owl:DatatypeProperty>
    


    <!-- http://seodwarf.eu/ontology/v1.0#hasOnlineResource -->

    <owl:DatatypeProperty rdf:about="http://seodwarf.eu/ontology/v1.0#hasOnlineResource">
        <rdfs:domain rdf:resource="http://seodwarf.eu/ontology/v1.0#SatelliteImage"/>
        <rdfs:range rdf:resource="http://www.w3.org/2001/XMLSchema#string"/>
        <rdfs:comment>It indicates the link for obtaining the resource from the
web. It accepts alphanumerical strings compatible with URL format as the “URL” property of the Dublin Core Ontology</rdfs:comment>
        <rdfs:isDefinedBy>dct:url</rdfs:isDefinedBy>
    </owl:DatatypeProperty>
    


    <!-- http://seodwarf.eu/ontology/v1.0#hasPhenomenonCoverage -->

    <owl:DatatypeProperty rdf:about="http://seodwarf.eu/ontology/v1.0#hasPhenomenonCoverage">
        <rdfs:domain rdf:resource="http://seodwarf.eu/ontology/v1.0#Phenomenon"/>
        <rdfs:range rdf:resource="http://www.w3.org/2001/XMLSchema#string"/>
        <rdfs:comment>The geometry of the phenomenon in WKT</rdfs:comment>
    </owl:DatatypeProperty>
    


    <!-- http://seodwarf.eu/ontology/v1.0#hasResponsible -->

    <owl:DatatypeProperty rdf:about="http://seodwarf.eu/ontology/v1.0#hasResponsible">
        <rdfs:domain rdf:resource="http://seodwarf.eu/ontology/v1.0#SatelliteImage"/>
        <rdfs:range rdf:resource="http://www.w3.org/2001/XMLSchema#string"/>
        <rdfs:comment>It describes the name of the subject responsible of the image.
It accepts alphanumerical values</rdfs:comment>
    </owl:DatatypeProperty>
    


    <!-- http://seodwarf.eu/ontology/v1.0#hasSourceSatelliteName -->

    <owl:DatatypeProperty rdf:about="http://seodwarf.eu/ontology/v1.0#hasSourceSatelliteName">
        <rdf:type rdf:resource="http://www.w3.org/2002/07/owl#FunctionalProperty"/>
        <rdfs:domain rdf:resource="http://seodwarf.eu/ontology/v1.0#SatelliteImage"/>
        <rdfs:range>
            <rdfs:Datatype>
                <owl:oneOf>
                    <rdf:Description>
                        <rdf:type rdf:resource="http://www.w3.org/1999/02/22-rdf-syntax-ns#List"/>
                        <rdf:first>Sentinel 1</rdf:first>
                        <rdf:rest>
                            <rdf:Description>
                                <rdf:type rdf:resource="http://www.w3.org/1999/02/22-rdf-syntax-ns#List"/>
                                <rdf:first>Sentinel 2</rdf:first>
                                <rdf:rest>
                                    <rdf:Description>
                                        <rdf:type rdf:resource="http://www.w3.org/1999/02/22-rdf-syntax-ns#List"/>
                                        <rdf:first>Sentinel 3</rdf:first>
                                        <rdf:rest rdf:resource="http://www.w3.org/1999/02/22-rdf-syntax-ns#nil"/>
                                    </rdf:Description>
                                </rdf:rest>
                            </rdf:Description>
                        </rdf:rest>
                    </rdf:Description>
                </owl:oneOf>
            </rdfs:Datatype>
        </rdfs:range>
        <rdfs:comment>It describes the name of the satellite from which the
image came from. It accepts one of the following textual values: “Sentinel 1”,
“Sentinel 2”, “Sentinel 3”. It is defined as the “source” property of the Dublin Core
Ontology</rdfs:comment>
        <rdfs:isDefinedBy>dct:source</rdfs:isDefinedBy>
    </owl:DatatypeProperty>
    


    <!-- http://seodwarf.eu/ontology/v1.0#hasSpatialResolution -->

    <owl:DatatypeProperty rdf:about="http://seodwarf.eu/ontology/v1.0#hasSpatialResolution">
        <rdf:type rdf:resource="http://www.w3.org/2002/07/owl#FunctionalProperty"/>
        <rdfs:domain rdf:resource="http://seodwarf.eu/ontology/v1.0#SatelliteImage"/>
        <rdfs:range rdf:resource="http://www.w3.org/2001/XMLSchema#integer"/>
        <rdfs:comment>It describes the presence of a resolution value for the
image. It accepts numerical values and it is defined as a generic RDF property</rdfs:comment>
    </owl:DatatypeProperty>
    


    <!-- http://seodwarf.eu/ontology/v1.0#hasTimestamp -->

    <owl:DatatypeProperty rdf:about="http://seodwarf.eu/ontology/v1.0#hasTimestamp">
        <rdfs:range rdf:resource="http://www.w3.org/2001/XMLSchema#long"/>
        <rdfs:comment>It describes the timestamp of acquisition of the image. It is
defined as the “temporal” property of the Dublin Core Ontology</rdfs:comment>
        <rdfs:isDefinedBy>dct:temporal</rdfs:isDefinedBy>
    </owl:DatatypeProperty>
    


    <!-- http://seodwarf.eu/ontology/v1.0#hasTitle -->

    <owl:DatatypeProperty rdf:about="http://seodwarf.eu/ontology/v1.0#hasTitle">
        <rdf:type rdf:resource="http://www.w3.org/2002/07/owl#FunctionalProperty"/>
        <rdfs:domain rdf:resource="http://seodwarf.eu/ontology/v1.0#SatelliteImage"/>
        <rdfs:range rdf:resource="http://www.w3.org/2001/XMLSchema#string"/>
        <rdfs:comment>It describes the title assigned to the image. It accepts alphanumerical
values and it is defined as the “title” property of the Dublin Core Ontology.</rdfs:comment>
        <rdfs:isDefinedBy>dct:title</rdfs:isDefinedBy>
    </owl:DatatypeProperty>
    


    <!-- http://seodwarf.eu/ontology/v1.0#hasType -->

    <owl:DatatypeProperty rdf:about="http://seodwarf.eu/ontology/v1.0#hasType">
        <rdfs:domain rdf:resource="http://seodwarf.eu/ontology/v1.0#SatelliteImage"/>
        <rdfs:range rdf:resource="http://www.w3.org/2001/XMLSchema#string"/>
        <rdfs:comment>It describes the representation type of the image. It accepts
alphanumerical values</rdfs:comment>
    </owl:DatatypeProperty>
    


    <!-- 
    ///////////////////////////////////////////////////////////////////////////////////////
    //
    // Classes
    //
    ///////////////////////////////////////////////////////////////////////////////////////
     -->

    


    <!-- http://seodwarf.eu/ontology/v1.0#AlgalBloom -->

    <owl:Class rdf:about="http://seodwarf.eu/ontology/v1.0#AlgalBloom">
        <rdfs:subClassOf rdf:resource="http://seodwarf.eu/ontology/v1.0#OceanPhenomenon"/>
        <rdfs:comment>it refers to the rapid increase or accumulation in the population of algae in
a water system. The concept is placed as subclass of “seo:ocean_phenomenon” but it
is linked with the SWEET Ontology concept “algal bloom” and with the DBpedia concept
“Algal_Bloom”</rdfs:comment>
        <rdfs:seeAlso>dbo:Algal_Bloom</rdfs:seeAlso>
        <rdfs:seeAlso>swe:AlgalBloom</rdfs:seeAlso>
    </owl:Class>
    


    <!-- http://seodwarf.eu/ontology/v1.0#Front -->

    <owl:Class rdf:about="http://seodwarf.eu/ontology/v1.0#Front">
        <rdfs:subClassOf rdf:resource="http://seodwarf.eu/ontology/v1.0#OceanPhenomenon"/>
        <rdfs:comment>it refers to a boundary separating two water masses moving in two different
directions. The concept is placed as subclass of “seo:ocean_phenomenon” and it is
linked the DBpedia concept “Front_(oceanography)</rdfs:comment>
        <rdfs:seeAlso>dbo:Front(Oceanography)</rdfs:seeAlso>
    </owl:Class>
    


    <!-- http://seodwarf.eu/ontology/v1.0#HotSpot -->

    <owl:Class rdf:about="http://seodwarf.eu/ontology/v1.0#HotSpot">
        <rdfs:subClassOf rdf:resource="http://seodwarf.eu/ontology/v1.0#OceanPhenomenon"/>
        <rdfs:comment>It is an area with higher water temperature than the temperatures recorded
usually</rdfs:comment>
    </owl:Class>
    


    <!-- http://seodwarf.eu/ontology/v1.0#Image -->

    <owl:Class rdf:about="http://seodwarf.eu/ontology/v1.0#Image">
        <rdfs:subClassOf rdf:resource="http://seodwarf.eu/ontology/v1.0#SatelliteImage"/>
        <rdfs:comment>The concept refers to a satellite image, used and archived in the project. It is the
source used for responding to the user queries. Searching in the SWEET Ontology, we
can identify the concept of “image” under the “Representation” class. The concept of
“image” is extended generating the class of “Satellite Image” and the class “seo:image”</rdfs:comment>
    </owl:Class>
    


    <!-- http://seodwarf.eu/ontology/v1.0#OceanPhenomenon -->

    <owl:Class rdf:about="http://seodwarf.eu/ontology/v1.0#OceanPhenomenon">
        <rdfs:subClassOf rdf:resource="http://seodwarf.eu/ontology/v1.0#Phenomenon"/>
        <rdfs:seeAlso>swe:OceanPhenomena</rdfs:seeAlso>
    </owl:Class>
    


    <!-- http://seodwarf.eu/ontology/v1.0#OilSpill -->

    <owl:Class rdf:about="http://seodwarf.eu/ontology/v1.0#OilSpill">
        <rdfs:subClassOf rdf:resource="http://seodwarf.eu/ontology/v1.0#OceanPhenomenon"/>
        <rdfs:comment>It refers to areas where liquid petroleum is released into the environment,
especially marine areas. The concept is placed as subclass of “seo:ocean_phenomenon”
but it is linked with the SWEET Ontology concept “oil spill” and with the DBpedia concept
“Oil_spill”</rdfs:comment>
        <rdfs:seeAlso>dbo:Oil_spill</rdfs:seeAlso>
        <rdfs:seeAlso>swe:Oil_Spill</rdfs:seeAlso>
    </owl:Class>
    


    <!-- http://seodwarf.eu/ontology/v1.0#Phenomenon -->

    <owl:Class rdf:about="http://seodwarf.eu/ontology/v1.0#Phenomenon">
        <rdfs:comment>The general concept “phenomenon” is specialized into the
“ocean_phenomenon” and where possible, concepts and relations from other ontologies
are reused, while new concepts and relations are added if required. It refers to the
DBpedia concept “Phenomenon” for creating a linking point with the Linked Open Data
Cloud</rdfs:comment>
        <rdfs:seeAlso>swe:PlanetaryPhenomena</rdfs:seeAlso>
    </owl:Class>
    


    <!-- http://seodwarf.eu/ontology/v1.0#SatelliteImage -->

    <owl:Class rdf:about="http://seodwarf.eu/ontology/v1.0#SatelliteImage">
        <rdfs:seeAlso>dbo:Satellite_imagery</rdfs:seeAlso>
    </owl:Class>
    


    <!-- http://seodwarf.eu/ontology/v1.0#ShallowWater -->

    <owl:Class rdf:about="http://seodwarf.eu/ontology/v1.0#ShallowWater">
        <rdfs:subClassOf rdf:resource="http://seodwarf.eu/ontology/v1.0#OceanPhenomenon"/>
        <rdfs:comment>it refers to phenomenon about the disruption of the natural orbital motion
of the wind. The concept is placed as subclass of “seo:ocean_phenomenon” and it is
linked the DBpedia concept “Waves_and_shallow_water”</rdfs:comment>
        <rdfs:seeAlso>dbo:Waves_and_Shallow_Water</rdfs:seeAlso>
    </owl:Class>
    


    <!-- http://seodwarf.eu/ontology/v1.0#TrophicStatusIndex -->

    <owl:Class rdf:about="http://seodwarf.eu/ontology/v1.0#TrophicStatusIndex">
        <rdfs:subClassOf rdf:resource="http://seodwarf.eu/ontology/v1.0#OceanPhenomenon"/>
        <rdfs:comment>It refers to the increase of nutrient concentrations followed by
corollary increases in subsequent trophic levels, such as eutrophication. The concept is
placed as subclass of “seo:ocean_phenomenon” and it is linked the DBpedia concept
“Trophic_state_index”</rdfs:comment>
        <rdfs:seeAlso>dbo:Trophic_state_index</rdfs:seeAlso>
    </owl:Class>
    


    <!-- http://seodwarf.eu/ontology/v1.0#Turbidity -->

    <owl:Class rdf:about="http://seodwarf.eu/ontology/v1.0#Turbidity">
        <rdfs:subClassOf rdf:resource="http://seodwarf.eu/ontology/v1.0#OceanPhenomenon"/>
        <rdfs:comment>it refers to the cloudiness or haziness of a fluid caused by large numbers of
individual particles. The concept is placed as subclass of “seo:ocean_phenomenon” but
it is linked with the SWEET Ontology concept “Turbidity” and with the DBpedia concept
“Turbidity”</rdfs:comment>
        <rdfs:seeAlso>dbo:Oil_Spill</rdfs:seeAlso>
        <rdfs:seeAlso>swe:OilSpill</rdfs:seeAlso>
    </owl:Class>
    


    <!-- http://seodwarf.eu/ontology/v1.0#Upwelling -->

    <owl:Class rdf:about="http://seodwarf.eu/ontology/v1.0#Upwelling">
        <rdfs:subClassOf rdf:resource="http://seodwarf.eu/ontology/v1.0#OceanPhenomenon"/>
        <rdfs:comment>It refers to areas where water with Sea Surface Temperature (SST) lower
than surrounding one is recorded. The concept is placed as subclass of
“seo:ocean_phenomenon” but it is linked with the SWEET Ontology concept “Upwelling”
and with the DBpedia concept “Upwelling”</rdfs:comment>
        <rdfs:seeAlso>dbo:Upwelling</rdfs:seeAlso>
        <rdfs:seeAlso>swe:Upwelling</rdfs:seeAlso>
    </owl:Class>
    


    <!-- http://seodwarf.eu/ontology/v1.0#Wave -->

    <owl:Class rdf:about="http://seodwarf.eu/ontology/v1.0#Wave">
        <rdfs:subClassOf rdf:resource="http://seodwarf.eu/ontology/v1.0#OceanPhenomenon"/>
        <rdfs:comment>it refers to the waves present on the sea surfaces. The concept is placed as
subclass of “seo:ocean_phenomenon” and it is linked the DBpedia concept
“Wind_wave”</rdfs:comment>
        <rdfs:seeAlso>dbo:Wind_Wave</rdfs:seeAlso>
    </owl:Class>
    


    <!-- http://seodwarf.eu/ontology/v1.0#Wind -->

    <owl:Class rdf:about="http://seodwarf.eu/ontology/v1.0#Wind">
        <rdfs:subClassOf rdf:resource="http://seodwarf.eu/ontology/v1.0#OceanPhenomenon"/>
        <rdfs:comment>the concept refers to a sea surface wind that is a crucial parameter for operational
use and for studies in coastal regions. The concept is placed as subclass of
“seo:ocean_phenomenon” and it is linked with the SWEET Ontology concept “Ocean
Wind” and with the DBpedia concept “Wind”</rdfs:comment>
        <rdfs:seeAlso>dbo:Wind</rdfs:seeAlso>
        <rdfs:seeAlso>swe:OceanWind</rdfs:seeAlso>
    </owl:Class>
    


    <!-- 
    ///////////////////////////////////////////////////////////////////////////////////////
    //
    // General axioms
    //
    ///////////////////////////////////////////////////////////////////////////////////////
     -->

    <rdf:Description>
        <rdf:type rdf:resource="http://www.w3.org/2002/07/owl#AllDisjointClasses"/>
        <owl:members rdf:parseType="Collection">
            <rdf:Description rdf:about="http://seodwarf.eu/ontology/v1.0#AlgalBloom"/>
            <rdf:Description rdf:about="http://seodwarf.eu/ontology/v1.0#Front"/>
            <rdf:Description rdf:about="http://seodwarf.eu/ontology/v1.0#HotSpot"/>
            <rdf:Description rdf:about="http://seodwarf.eu/ontology/v1.0#OilSpill"/>
            <rdf:Description rdf:about="http://seodwarf.eu/ontology/v1.0#ShallowWater"/>
            <rdf:Description rdf:about="http://seodwarf.eu/ontology/v1.0#TrophicStatusIndex"/>
            <rdf:Description rdf:about="http://seodwarf.eu/ontology/v1.0#Turbidity"/>
            <rdf:Description rdf:about="http://seodwarf.eu/ontology/v1.0#Upwelling"/>
            <rdf:Description rdf:about="http://seodwarf.eu/ontology/v1.0#Wave"/>
            <rdf:Description rdf:about="http://seodwarf.eu/ontology/v1.0#Wind"/>
        </owl:members>
    </rdf:Description>
</rdf:RDF>



<!-- Generated by the OWL API (version 4.2.6.20160910-2108) https://github.com/owlcs/owlapi -->

