<?xml version="1.0"?>
<rdf:RDF xmlns="http://seodwarf.eu/ontology/v1.0#"
     xml:base="http://seodwarf.eu/ontology/v1.0"
     xmlns:swe="https://sweet.jpl.nasa.gov/sweet2.3/"
     xmlns:owl="http://www.w3.org/2002/07/owl#"
     xmlns:gn="http://www.geonames.org/ontology"
     xmlns:xsd="http://www.w3.org/2001/XMLSchema#"
     xmlns:rdfs="http://www.w3.org/2000/01/rdf-schema#"
     xmlns:dbo="http://dbpedia.org/resource/"
     xmlns:geo="http://www.eionet.europa.eu/gemet"
     xmlns:dct="http://dublincore.org/documents/2012/06/14/dcmiterms/"
     xmlns:rdf="http://www.w3.org/1999/02/22-rdf-syntax-ns#"
     xmlns:xml="http://www.w3.org/XML/1998/namespace"
     xmlns:strdf="http://strdf.di.uoa.gr/ontology/"
     xmlns:seo="http://seodwarf.eu/ontology/v1.0">
    <owl:Ontology rdf:about="http://seodwarf.eu/ontology/v1.0">
        <owl:versionIRI rdf:resource="http://seodwarf.eu/ontology/v1.0/1.0.0"/>
        <owl:imports rdf:resource="http://sweet.jpl.nasa.gov/2.3/sweetAll.owl"/>
        <rdfs:label>SEO-DWARF Environment Ontology</rdfs:label>
    </owl:Ontology>
    


    <!-- 
    ///////////////////////////////////////////////////////////////////////////////////////
    //
    // Object Properties
    //
    ///////////////////////////////////////////////////////////////////////////////////////
     -->

    


    <!-- http://seodwarf.eu/ontology/v1.0#hasAdministrativeRegion -->

    <owl:ObjectProperty rdf:about="http://seodwarf.eu/ontology/v1.0#hasAdministrativeRegion">
        <rdfs:domain rdf:resource="http://seodwarf.eu/ontology/v1.0#ImageContentArea"/>
        <rdfs:range rdf:resource="http://sweet.jpl.nasa.gov/2.3/humanJurisdiction.owl#AdministrativeRegion"/>
        <rdfs:comment>It describes the reference of the area to an
institutional region such as a Country, Region, Province, City that has the
administrative power on the region defined. It refers to the “administrative_region”
concept. It is defined as a generic RDF property.</rdfs:comment>
    </owl:ObjectProperty>
    


    <!-- http://seodwarf.eu/ontology/v1.0#hasAlgae -->

    <owl:ObjectProperty rdf:about="http://seodwarf.eu/ontology/v1.0#hasAlgae">
        <rdfs:domain rdf:resource="http://seodwarf.eu/ontology/v1.0#AlgalBloom"/>
        <rdfs:range rdf:resource="http://seodwarf.eu/ontology/v1.0#Algae"/>
        <rdfs:comment>I refers to the algae identified for the bloom. The properties has the
“seo:algae” class as a range.</rdfs:comment>
    </owl:ObjectProperty>
    


    <!-- http://seodwarf.eu/ontology/v1.0#hasBodyOfWater -->

    <owl:ObjectProperty rdf:about="http://seodwarf.eu/ontology/v1.0#hasBodyOfWater">
        <rdfs:domain rdf:resource="http://seodwarf.eu/ontology/v1.0#Front"/>
        <rdfs:range rdf:resource="http://sweet.jpl.nasa.gov/2.3/realmHydroBody.owl#BodyOfWater"/>
        <rdfs:comment>It describes the presence of the two different water masses
that mover in different directions and that have different properties.</rdfs:comment>
    </owl:ObjectProperty>
    


    <!-- http://seodwarf.eu/ontology/v1.0#hasCapturingDate -->

    <owl:ObjectProperty rdf:about="http://seodwarf.eu/ontology/v1.0#hasCapturingDate">
        <rdf:type rdf:resource="http://www.w3.org/2002/07/owl#FunctionalProperty"/>
        <rdfs:domain rdf:resource="http://seodwarf.eu/ontology/v1.0#SatelliteImage"/>
        <rdfs:range rdf:resource="http://sweet.jpl.nasa.gov/2.3/propTime.owl#Time"/>
        <rdfs:comment>It describes the presence of the acquisition date of the
image. It refers to the “Time” concept of SWEET Ontology, and It is defined as the
“temporal” property of the Dublin Core Ontology</rdfs:comment>
        <rdfs:isDefinedBy>dct:temporal</rdfs:isDefinedBy>
    </owl:ObjectProperty>
    


    <!-- http://seodwarf.eu/ontology/v1.0#hasCardinalDirection -->

    <owl:ObjectProperty rdf:about="http://seodwarf.eu/ontology/v1.0#hasCardinalDirection">
        <rdfs:domain>
            <owl:Class>
                <owl:unionOf rdf:parseType="Collection">
                    <rdf:Description rdf:about="http://seodwarf.eu/ontology/v1.0#Wind"/>
                    <rdf:Description rdf:about="http://sweet.jpl.nasa.gov/2.3/realmHydroBody.owl#BodyOfWater"/>
                </owl:unionOf>
            </owl:Class>
        </rdfs:domain>
        <rdfs:range rdf:resource="http://seodwarf.eu/ontology/v1.0#CardinalDirection"/>
        <rdfs:comment>It refers to the cardinal direction. The
properties has the “seo:cardinal_direction” class as a range</rdfs:comment>
    </owl:ObjectProperty>
    


    <!-- http://seodwarf.eu/ontology/v1.0#hasChlorophyllConcentration -->

    <owl:ObjectProperty rdf:about="http://seodwarf.eu/ontology/v1.0#hasChlorophyllConcentration">
        <rdfs:domain>
            <owl:Class>
                <owl:unionOf rdf:parseType="Collection">
                    <rdf:Description rdf:about="http://seodwarf.eu/ontology/v1.0#AlgalBloom"/>
                    <rdf:Description rdf:about="http://seodwarf.eu/ontology/v1.0#TrophicStatusIndex"/>
                    <rdf:Description rdf:about="http://seodwarf.eu/ontology/v1.0#Upwelling"/>
                    <rdf:Description rdf:about="http://sweet.jpl.nasa.gov/2.3/realmHydroBody.owl#BodyOfWater"/>
                </owl:unionOf>
            </owl:Class>
        </rdfs:domain>
        <rdfs:range rdf:resource="http://seodwarf.eu/ontology/v1.0#ChlorophyllConcentration"/>
        <rdfs:comment>It refers to the chlorophyll concentration in the
area. The properties has the
“seo:chlorophyll_concentration” class as a range</rdfs:comment>
    </owl:ObjectProperty>
    


    <!-- http://seodwarf.eu/ontology/v1.0#hasContentArea -->

    <owl:ObjectProperty rdf:about="http://seodwarf.eu/ontology/v1.0#hasContentArea">
        <rdfs:domain rdf:resource="http://seodwarf.eu/ontology/v1.0#SatelliteImage"/>
        <rdfs:range rdf:resource="http://seodwarf.eu/ontology/v1.0#ImageContentArea"/>
        <rdfs:comment>It describes the presence of different relevant areas in the
image. It refers to the “seo:image_ content_area” concept and It is defined as the
“hasPart” property of the Dublin Core Ontology</rdfs:comment>
        <rdfs:isDefinedBy>dct:hasPart</rdfs:isDefinedBy>
    </owl:ObjectProperty>
    


    <!-- http://seodwarf.eu/ontology/v1.0#hasCoverage -->

    <owl:ObjectProperty rdf:about="http://seodwarf.eu/ontology/v1.0#hasCoverage">
        <rdfs:domain>
            <owl:Class>
                <owl:unionOf rdf:parseType="Collection">
                    <rdf:Description rdf:about="http://seodwarf.eu/ontology/v1.0#ImageContentArea"/>
                    <rdf:Description rdf:about="http://seodwarf.eu/ontology/v1.0#SatelliteImage"/>
                </owl:unionOf>
            </owl:Class>
        </rdfs:domain>
        <rdfs:range rdf:resource="http://seodwarf.eu/ontology/v1.0#GeographicalCoordinate"/>
        <rdfs:comment>It describes the spatial coverage of the image or the image content region. It refers to the
“geographical_coordinate” concept. It is defined as the “coverage” property of the
Dublin Core Ontology</rdfs:comment>
        <rdfs:isDefinedBy>dct:coverage</rdfs:isDefinedBy>
    </owl:ObjectProperty>
    


    <!-- http://seodwarf.eu/ontology/v1.0#hasDistanceFromCoast -->

    <owl:ObjectProperty rdf:about="http://seodwarf.eu/ontology/v1.0#hasDistanceFromCoast">
        <rdfs:domain rdf:resource="http://seodwarf.eu/ontology/v1.0#OilSpill"/>
        <rdfs:range rdf:resource="http://sweet.jpl.nasa.gov/2.3/propSpaceDistance.owl#Distance"/>
        <rdfs:comment>It refers to the distance from the coast of the spill.
The properties has the “swe:Distance” class as a range. It is measured in Km</rdfs:comment>
    </owl:ObjectProperty>
    


    <!-- http://seodwarf.eu/ontology/v1.0#hasHeight -->

    <owl:ObjectProperty rdf:about="http://seodwarf.eu/ontology/v1.0#hasHeight">
        <rdfs:domain rdf:resource="http://seodwarf.eu/ontology/v1.0#Wave"/>
        <rdfs:range rdf:resource="http://sweet.jpl.nasa.gov/2.3/propSpaceHeight.owl#Height"/>
        <rdfs:comment>It refers to the height of the wave. The properties has the “swe:heght”
class as a range</rdfs:comment>
    </owl:ObjectProperty>
    


    <!-- http://seodwarf.eu/ontology/v1.0#hasPhenomenon -->

    <owl:ObjectProperty rdf:about="http://seodwarf.eu/ontology/v1.0#hasPhenomenon">
        <rdf:type rdf:resource="http://www.w3.org/2002/07/owl#FunctionalProperty"/>
        <rdfs:domain rdf:resource="http://seodwarf.eu/ontology/v1.0#ImageContentArea"/>
        <rdfs:range rdf:resource="http://seodwarf.eu/ontology/v1.0#Phenomenon"/>
        <rdfs:comment>It describes the phenomenon present in the region of
reference. It refers to the “image_SEO-DWARF_phenomenon” concept. It is
defined as the “Part” property of the Dublin Core Ontology</rdfs:comment>
        <rdfs:isDefinedBy>dct:hasPart</rdfs:isDefinedBy>
    </owl:ObjectProperty>
    


    <!-- http://seodwarf.eu/ontology/v1.0#hasPhenomenonCoverage -->

    <owl:ObjectProperty rdf:about="http://seodwarf.eu/ontology/v1.0#hasPhenomenonCoverage">
        <rdfs:domain rdf:resource="http://seodwarf.eu/ontology/v1.0#Phenomenon"/>
        <rdfs:range rdf:resource="http://seodwarf.eu/ontology/v1.0#GeographicalCoordinate"/>
        <rdfs:comment>It describes the spatial coverage of the
phenomenon. It refers to the “geographical_coordinate” concept. It is defined as
the “coverage” property of the Dublin Core Ontology</rdfs:comment>
        <rdfs:isDefinedBy>dct:coverage</rdfs:isDefinedBy>
    </owl:ObjectProperty>
    


    <!-- http://seodwarf.eu/ontology/v1.0#hasRate -->

    <owl:ObjectProperty rdf:about="http://seodwarf.eu/ontology/v1.0#hasRate">
        <rdfs:domain rdf:resource="http://seodwarf.eu/ontology/v1.0#Wave"/>
        <rdfs:comment>It refers to the rate of the wave. The properties has the “swe:rate” class
as a range</rdfs:comment>
    </owl:ObjectProperty>
    


    <!-- http://seodwarf.eu/ontology/v1.0#hasRegionType -->

    <owl:ObjectProperty rdf:about="http://seodwarf.eu/ontology/v1.0#hasRegionType">
        <rdfs:domain rdf:resource="http://seodwarf.eu/ontology/v1.0#ImageContentArea"/>
        <rdfs:range rdf:resource="http://seodwarf.eu/ontology/v1.0#RegionType"/>
        <rdfs:comment>It describes the type of the region (Sea, Lake, …). The list of elements
to use is obtained from the GEMET thesaurus. It will refer to the “content_type”
concept. It is defined as the “type” property of the Dublin Core Ontology.</rdfs:comment>
        <rdfs:isDefinedBy>dct:hasType</rdfs:isDefinedBy>
    </owl:ObjectProperty>
    


    <!-- http://seodwarf.eu/ontology/v1.0#hasSeaLevel -->

    <owl:ObjectProperty rdf:about="http://seodwarf.eu/ontology/v1.0#hasSeaLevel">
        <rdfs:domain>
            <owl:Class>
                <owl:unionOf rdf:parseType="Collection">
                    <rdf:Description rdf:about="http://seodwarf.eu/ontology/v1.0#Upwelling"/>
                    <rdf:Description rdf:about="http://sweet.jpl.nasa.gov/2.3/realmHydroBody.owl#BodyOfWater"/>
                </owl:unionOf>
            </owl:Class>
        </rdfs:domain>
        <rdfs:range rdf:resource="http://sweet.jpl.nasa.gov/2.3/propSpaceHeight.owl#SeaLevel"/>
        <rdfs:comment>It refers to the sea level . The properties has the
“swe:Sea Level” extended class as a range</rdfs:comment>
    </owl:ObjectProperty>
    


    <!-- http://seodwarf.eu/ontology/v1.0#hasSize -->

    <owl:ObjectProperty rdf:about="http://seodwarf.eu/ontology/v1.0#hasSize">
        <rdfs:domain rdf:resource="http://seodwarf.eu/ontology/v1.0#OilSpill"/>
        <rdfs:range rdf:resource="http://sweet.jpl.nasa.gov/2.3/propSpaceDistance.owl#Size"/>
        <rdfs:comment>it refers to the size of the spill. The properties has the “swe:Size” class
as a range. It is measured in m2</rdfs:comment>
    </owl:ObjectProperty>
    


    <!-- http://seodwarf.eu/ontology/v1.0#hasTemperature -->

    <owl:ObjectProperty rdf:about="http://seodwarf.eu/ontology/v1.0#hasTemperature">
        <rdfs:domain>
            <owl:Class>
                <owl:unionOf rdf:parseType="Collection">
                    <rdf:Description rdf:about="http://seodwarf.eu/ontology/v1.0#AlgalBloom"/>
                    <rdf:Description rdf:about="http://seodwarf.eu/ontology/v1.0#HotSpot"/>
                    <rdf:Description rdf:about="http://seodwarf.eu/ontology/v1.0#Upwelling"/>
                    <rdf:Description rdf:about="http://sweet.jpl.nasa.gov/2.3/realmHydroBody.owl#BodyOfWater"/>
                </owl:unionOf>
            </owl:Class>
        </rdfs:domain>
        <rdfs:range rdf:resource="http://sweet.jpl.nasa.gov/2.3/propTemperature.owl#Temperature"/>
        <rdfs:comment>it refers to the “swe:Temperature” concept and identify the
presence of one or more temperature measurement. It is
defined such as a standard RDF property</rdfs:comment>
    </owl:ObjectProperty>
    


    <!-- http://seodwarf.eu/ontology/v1.0#hasTotalSuspendedSoil -->

    <owl:ObjectProperty rdf:about="http://seodwarf.eu/ontology/v1.0#hasTotalSuspendedSoil">
        <rdfs:domain rdf:resource="http://seodwarf.eu/ontology/v1.0#ShallowWater"/>
        <rdfs:range rdf:resource="http://sweet.jpl.nasa.gov/2.3/propChemical.owl#TotalSuspendedSolids"/>
        <rdfs:comment>It refers to the quantity of total suspended matter on
the sea surface. The properties has the “swe:total_suspended_solid” class as a
range</rdfs:comment>
    </owl:ObjectProperty>
    


    <!-- http://strdf.di.uoa.gr/ontology/hasGeometry -->

    <owl:ObjectProperty rdf:about="http://strdf.di.uoa.gr/ontology/hasGeometry">
        <rdfs:domain rdf:resource="http://seodwarf.eu/ontology/v1.0#GeographicalCoordinate"/>
    </owl:ObjectProperty>
    


    <!-- http://sweet.jpl.nasa.gov/2.3/relaPhysical.owl#hasSpeed -->

    <rdf:Description rdf:about="http://sweet.jpl.nasa.gov/2.3/relaPhysical.owl#hasSpeed">
        <rdfs:domain>
            <owl:Class>
                <owl:unionOf rdf:parseType="Collection">
                    <rdf:Description rdf:about="http://seodwarf.eu/ontology/v1.0#OilSpill"/>
                    <rdf:Description rdf:about="http://seodwarf.eu/ontology/v1.0#Wind"/>
                </owl:unionOf>
            </owl:Class>
        </rdfs:domain>
        <rdfs:range rdf:resource="http://sweet.jpl.nasa.gov/2.3/propSpeed.owl#Speed"/>
    </rdf:Description>
    


    <!-- http://sweet.jpl.nasa.gov/2.3/relaTime.owl#hasEnd -->

    <rdf:Description rdf:about="http://sweet.jpl.nasa.gov/2.3/relaTime.owl#hasEnd">
        <rdfs:domain rdf:resource="http://seodwarf.eu/ontology/v1.0#Phenomenon"/>
    </rdf:Description>
    


    <!-- http://sweet.jpl.nasa.gov/2.3/relaTime.owl#hasStart -->

    <rdf:Description rdf:about="http://sweet.jpl.nasa.gov/2.3/relaTime.owl#hasStart">
        <rdfs:domain rdf:resource="http://seodwarf.eu/ontology/v1.0#Phenomenon"/>
    </rdf:Description>
    


    <!-- 
    ///////////////////////////////////////////////////////////////////////////////////////
    //
    // Data properties
    //
    ///////////////////////////////////////////////////////////////////////////////////////
     -->

    


    <!-- http://seodwarf.eu/ontology/v1.0#hasAbstract -->

    <owl:DatatypeProperty rdf:about="http://seodwarf.eu/ontology/v1.0#hasAbstract">
        <rdfs:domain rdf:resource="http://seodwarf.eu/ontology/v1.0#SatelliteImage"/>
        <rdfs:range rdf:resource="http://www.w3.org/2001/XMLSchema#string"/>
        <rdfs:comment>It describes the presence of a text description of the image. It
accepts alphanumerical values and it is defined as “abstract” property of the Dublin
Core Ontology</rdfs:comment>
        <rdfs:isDefinedBy>dct:abstract</rdfs:isDefinedBy>
    </owl:DatatypeProperty>
    


    <!-- http://seodwarf.eu/ontology/v1.0#hasAccuracy -->

    <owl:DatatypeProperty rdf:about="http://seodwarf.eu/ontology/v1.0#hasAccuracy">
        <rdf:type rdf:resource="http://www.w3.org/2002/07/owl#FunctionalProperty"/>
        <rdfs:domain rdf:resource="http://seodwarf.eu/ontology/v1.0#Phenomenon"/>
        <rdfs:range rdf:resource="http://www.w3.org/2001/XMLSchema#float"/>
        <rdfs:comment>It describes the accuracy of the phenomenon detected. It accepts
floating numbers values and is defined as a standard RDF property</rdfs:comment>
    </owl:DatatypeProperty>
    


    <!-- http://seodwarf.eu/ontology/v1.0#hasCardinalValue -->

    <owl:DatatypeProperty rdf:about="http://seodwarf.eu/ontology/v1.0#hasCardinalValue">
        <rdfs:domain rdf:resource="http://seodwarf.eu/ontology/v1.0#CardinalDirection"/>
        <rdfs:range rdf:resource="http://www.w3.org/2001/XMLSchema#integer"/>
        <rdfs:comment>It refers to the cardinal degree of the vector. It accepts integer
numbers as range</rdfs:comment>
    </owl:DatatypeProperty>
    


    <!-- http://seodwarf.eu/ontology/v1.0#hasChlorophyllAValue -->

    <owl:DatatypeProperty rdf:about="http://seodwarf.eu/ontology/v1.0#hasChlorophyllAValue">
        <rdfs:domain rdf:resource="http://seodwarf.eu/ontology/v1.0#ChlorophyllConcentration"/>
        <rdfs:range rdf:resource="http://www.w3.org/2001/XMLSchema#float"/>
        <rdfs:comment>It refers to the value of the measurement of the
chlorophyll a concentration. It accepts floating point numbers as range</rdfs:comment>
    </owl:DatatypeProperty>
    


    <!-- http://seodwarf.eu/ontology/v1.0#hasColour -->

    <owl:DatatypeProperty rdf:about="http://seodwarf.eu/ontology/v1.0#hasColour">
        <rdfs:domain>
            <owl:Class>
                <owl:unionOf rdf:parseType="Collection">
                    <rdf:Description rdf:about="http://seodwarf.eu/ontology/v1.0#ShallowWater"/>
                    <rdf:Description rdf:about="http://seodwarf.eu/ontology/v1.0#Turbidity"/>
                    <rdf:Description rdf:about="http://sweet.jpl.nasa.gov/2.3/realmHydroBody.owl#BodyOfWater"/>
                </owl:unionOf>
            </owl:Class>
        </rdfs:domain>
        <rdfs:range rdf:resource="http://www.w3.org/2001/XMLSchema#string"/>
        <rdfs:comment>It refers to the water colour assigned to the instance . It
accepts string values and is defined as a standard RDF property</rdfs:comment>
    </owl:DatatypeProperty>
    


    <!-- http://seodwarf.eu/ontology/v1.0#hasEastLongitude -->

    <owl:DatatypeProperty rdf:about="http://seodwarf.eu/ontology/v1.0#hasEastLongitude">
        <rdf:type rdf:resource="http://www.w3.org/2002/07/owl#FunctionalProperty"/>
        <rdfs:domain rdf:resource="http://seodwarf.eu/ontology/v1.0#BoxCoordinate"/>
        <rdfs:range rdf:resource="http://www.w3.org/2001/XMLSchema#float"/>
        <rdfs:comment>It describes the east latitude of the map box. It accepts
float values in the range -180 +180. It is defined as a generic RDF property.</rdfs:comment>
    </owl:DatatypeProperty>
    


    <!-- http://seodwarf.eu/ontology/v1.0#hasFormat -->

    <owl:DatatypeProperty rdf:about="http://seodwarf.eu/ontology/v1.0#hasFormat">
        <rdfs:domain rdf:resource="http://seodwarf.eu/ontology/v1.0#SatelliteImage"/>
        <rdfs:range rdf:resource="http://www.w3.org/2001/XMLSchema#string"/>
        <rdfs:comment>It describes the format of the image (raster or raw). It accepts
alphanumerical values</rdfs:comment>
    </owl:DatatypeProperty>
    


    <!-- http://seodwarf.eu/ontology/v1.0#hasGEMETID -->

    <owl:DatatypeProperty rdf:about="http://seodwarf.eu/ontology/v1.0#hasGEMETID">
        <rdf:type rdf:resource="http://www.w3.org/2002/07/owl#FunctionalProperty"/>
        <rdfs:domain rdf:resource="http://seodwarf.eu/ontology/v1.0#RegionType"/>
        <rdfs:range rdf:resource="http://www.w3.org/2001/XMLSchema#integer"/>
        <rdfs:comment>It describes the GEMET id of the region type. It accepts
alphanumerical values and it is defined as the “identifier” property of the Dublin
Core Ontology</rdfs:comment>
        <rdfs:isDefinedBy>dct:identifier</rdfs:isDefinedBy>
    </owl:DatatypeProperty>
    


    <!-- http://seodwarf.eu/ontology/v1.0#hasGEMETName -->

    <owl:DatatypeProperty rdf:about="http://seodwarf.eu/ontology/v1.0#hasGEMETName">
        <rdf:type rdf:resource="http://www.w3.org/2002/07/owl#FunctionalProperty"/>
        <rdfs:domain rdf:resource="http://seodwarf.eu/ontology/v1.0#RegionType"/>
        <rdfs:range rdf:resource="http://www.w3.org/2001/XMLSchema#string"/>
        <rdfs:comment>It describes the name assigned to the region type in GEMET.
It accepts alphanumerical values and it is defined as the “title” property of the
Dublin Core Ontology</rdfs:comment>
        <rdfs:isDefinedBy>dct:title</rdfs:isDefinedBy>
    </owl:DatatypeProperty>
    


    <!-- http://seodwarf.eu/ontology/v1.0#hasGeonamesID -->

    <owl:DatatypeProperty rdf:about="http://seodwarf.eu/ontology/v1.0#hasGeonamesID">
        <rdf:type rdf:resource="http://www.w3.org/2002/07/owl#FunctionalProperty"/>
        <rdfs:domain rdf:resource="http://sweet.jpl.nasa.gov/2.3/humanJurisdiction.owl#AdministrativeRegion"/>
        <rdfs:range rdf:resource="http://www.w3.org/2001/XMLSchema#integer"/>
        <rdfs:comment>It defines the Geonames concept id of the administrative
region. It accepts alphanumerical values and it is defined as the “identifier”
property of the Dublin Core Ontology</rdfs:comment>
        <rdfs:isDefinedBy>dct:identifier</rdfs:isDefinedBy>
    </owl:DatatypeProperty>
    


    <!-- http://seodwarf.eu/ontology/v1.0#hasGeonamesName -->

    <owl:DatatypeProperty rdf:about="http://seodwarf.eu/ontology/v1.0#hasGeonamesName">
        <rdfs:domain rdf:resource="http://sweet.jpl.nasa.gov/2.3/humanJurisdiction.owl#AdministrativeRegion"/>
        <rdfs:range rdf:resource="http://www.w3.org/2001/XMLSchema#string"/>
        <rdfs:comment>It describes the name assigned to the administrative
region of interest in Geonames. It accepts alphanumerical values and is defined
as the “title” property in the Dublin Core Ontology</rdfs:comment>
        <rdfs:isDefinedBy>dct:title</rdfs:isDefinedBy>
    </owl:DatatypeProperty>
    


    <!-- http://seodwarf.eu/ontology/v1.0#hasHeightValue -->

    <owl:DatatypeProperty rdf:about="http://seodwarf.eu/ontology/v1.0#hasHeightValue">
        <rdfs:domain rdf:resource="http://sweet.jpl.nasa.gov/2.3/propSpaceHeight.owl#Height"/>
        <rdfs:range rdf:resource="http://www.w3.org/2001/XMLSchema#float"/>
        <rdfs:comment>It refers to the height of the wave. It accepts floating number
values and is defined as a standard RDF property</rdfs:comment>
    </owl:DatatypeProperty>
    


    <!-- http://seodwarf.eu/ontology/v1.0#hasIdentifier -->

    <owl:DatatypeProperty rdf:about="http://seodwarf.eu/ontology/v1.0#hasIdentifier">
        <rdf:type rdf:resource="http://www.w3.org/2002/07/owl#FunctionalProperty"/>
        <rdfs:domain rdf:resource="http://seodwarf.eu/ontology/v1.0#SatelliteImage"/>
        <rdfs:range rdf:resource="http://www.w3.org/2001/XMLSchema#string"/>
        <rdfs:comment>It describes presence of a unique identifier of the image in the
project. It accepts alphanumerical values and it is defined as the “identifier”
property of the Dublin Core Ontology.</rdfs:comment>
        <rdfs:isDefinedBy>dct:identifier</rdfs:isDefinedBy>
    </owl:DatatypeProperty>
    


    <!-- http://seodwarf.eu/ontology/v1.0#hasLatitude -->

    <owl:DatatypeProperty rdf:about="http://seodwarf.eu/ontology/v1.0#hasLatitude">
        <rdf:type rdf:resource="http://www.w3.org/2002/07/owl#FunctionalProperty"/>
        <rdfs:domain rdf:resource="http://seodwarf.eu/ontology/v1.0#PointCoordinate"/>
        <rdfs:range rdf:resource="http://www.w3.org/2001/XMLSchema#float"/>
        <rdfs:comment>It describes the latitude of the point on the map. It accepts float
values in the range -90 +90. It is defined as a generic RDF property</rdfs:comment>
    </owl:DatatypeProperty>
    


    <!-- http://seodwarf.eu/ontology/v1.0#hasLineage -->

    <owl:DatatypeProperty rdf:about="http://seodwarf.eu/ontology/v1.0#hasLineage">
        <rdfs:domain rdf:resource="http://seodwarf.eu/ontology/v1.0#SatelliteImage"/>
        <rdfs:range rdf:resource="http://www.w3.org/2001/XMLSchema#string"/>
        <rdfs:comment>It is a field containing different textual information about the image.
The content depends by the operator that fills it. It accepts alphanumerical values</rdfs:comment>
    </owl:DatatypeProperty>
    


    <!-- http://seodwarf.eu/ontology/v1.0#hasLongitude -->

    <owl:DatatypeProperty rdf:about="http://seodwarf.eu/ontology/v1.0#hasLongitude">
        <rdf:type rdf:resource="http://www.w3.org/2002/07/owl#FunctionalProperty"/>
        <rdfs:domain rdf:resource="http://seodwarf.eu/ontology/v1.0#PointCoordinate"/>
        <rdfs:range rdf:resource="http://www.w3.org/2001/XMLSchema#float"/>
        <rdfs:comment>It will describe the longitude of the map point. It will accept
float values in the range -180 +180. It is defined as a generic RDF property</rdfs:comment>
    </owl:DatatypeProperty>
    


    <!-- http://seodwarf.eu/ontology/v1.0#hasNorthLatitude -->

    <owl:DatatypeProperty rdf:about="http://seodwarf.eu/ontology/v1.0#hasNorthLatitude">
        <rdf:type rdf:resource="http://www.w3.org/2002/07/owl#FunctionalProperty"/>
        <rdfs:domain rdf:resource="http://seodwarf.eu/ontology/v1.0#BoxCoordinate"/>
        <rdfs:range rdf:resource="http://www.w3.org/2001/XMLSchema#float"/>
        <rdfs:comment>It describes the north latitude of the map box. It accepts
float values in the range -90 +90. It is defined as a generic RDF property.</rdfs:comment>
    </owl:DatatypeProperty>
    


    <!-- http://seodwarf.eu/ontology/v1.0#hasOnlineResource -->

    <owl:DatatypeProperty rdf:about="http://seodwarf.eu/ontology/v1.0#hasOnlineResource">
        <rdfs:domain rdf:resource="http://seodwarf.eu/ontology/v1.0#SatelliteImage"/>
        <rdfs:range rdf:resource="http://www.w3.org/2001/XMLSchema#string"/>
        <rdfs:comment>It indicates the link for obtaining the resource from the
web. It accepts alphanumerical strings compatible with URL format as the “URL” property of the Dublin Core Ontology</rdfs:comment>
        <rdfs:isDefinedBy>dct:url</rdfs:isDefinedBy>
    </owl:DatatypeProperty>
    


    <!-- http://seodwarf.eu/ontology/v1.0#hasRateValue -->

    <owl:DatatypeProperty rdf:about="http://seodwarf.eu/ontology/v1.0#hasRateValue">
        <rdfs:range rdf:resource="http://www.w3.org/2001/XMLSchema#float"/>
        <rdfs:comment>It refers to the rate of the wave. It accepts floating number values
and is defined as a standard RDF property</rdfs:comment>
    </owl:DatatypeProperty>
    


    <!-- http://seodwarf.eu/ontology/v1.0#hasRegionGeonamesID -->

    <owl:DatatypeProperty rdf:about="http://seodwarf.eu/ontology/v1.0#hasRegionGeonamesID">
        <rdfs:domain rdf:resource="http://seodwarf.eu/ontology/v1.0#ImageContentArea"/>
        <rdfs:range rdf:resource="http://www.w3.org/2001/XMLSchema#integer"/>
        <rdfs:comment>It describes the Geonames concept id available if
the area corresponds to a universal known region. It is defined as a generic RDF
property</rdfs:comment>
    </owl:DatatypeProperty>
    


    <!-- http://seodwarf.eu/ontology/v1.0#hasRegionName -->

    <owl:DatatypeProperty rdf:about="http://seodwarf.eu/ontology/v1.0#hasRegionName">
        <rdfs:domain rdf:resource="http://seodwarf.eu/ontology/v1.0#ImageContentArea"/>
        <rdfs:range rdf:resource="http://www.w3.org/2001/XMLSchema#string"/>
        <rdfs:comment>It describes the name assigned to the region of interest by
the user or the system that define the area. It accepts alphanumerical values and
it is defined as the “title” property of the Dublin Core Ontology</rdfs:comment>
        <rdfs:isDefinedBy>dct:title</rdfs:isDefinedBy>
    </owl:DatatypeProperty>
    


    <!-- http://seodwarf.eu/ontology/v1.0#hasResolution -->

    <owl:DatatypeProperty rdf:about="http://seodwarf.eu/ontology/v1.0#hasResolution">
        <rdfs:domain rdf:resource="http://seodwarf.eu/ontology/v1.0#SatelliteImage"/>
        <rdfs:range rdf:resource="http://www.w3.org/2001/XMLSchema#integer"/>
        <rdfs:comment>It describes the presence of a resolution value for the
image. It accepts numerical values and it is defined as a generic RDF property</rdfs:comment>
    </owl:DatatypeProperty>
    


    <!-- http://seodwarf.eu/ontology/v1.0#hasResponsible -->

    <owl:DatatypeProperty rdf:about="http://seodwarf.eu/ontology/v1.0#hasResponsible">
        <rdfs:domain rdf:resource="http://seodwarf.eu/ontology/v1.0#SatelliteImage"/>
        <rdfs:range rdf:resource="http://www.w3.org/2001/XMLSchema#string"/>
        <rdfs:comment>It describes the name of the subject responsible of the image.
It accepts alphanumerical values</rdfs:comment>
    </owl:DatatypeProperty>
    


    <!-- http://seodwarf.eu/ontology/v1.0#hasSeaLevelValue -->

    <owl:DatatypeProperty rdf:about="http://seodwarf.eu/ontology/v1.0#hasSeaLevelValue">
        <rdfs:domain rdf:resource="http://sweet.jpl.nasa.gov/2.3/propSpaceHeight.owl#SeaLevel"/>
        <rdfs:range rdf:resource="http://www.w3.org/2001/XMLSchema#float"/>
        <rdfs:comment>It refers to the value of the measurement of the sea level. It
accepts floating point numbers as range</rdfs:comment>
    </owl:DatatypeProperty>
    


    <!-- http://seodwarf.eu/ontology/v1.0#hasSeason -->

    <owl:DatatypeProperty rdf:about="http://seodwarf.eu/ontology/v1.0#hasSeason">
        <rdfs:domain rdf:resource="http://sweet.jpl.nasa.gov/2.3/propTime.owl#Time"/>
        <rdfs:range>
            <rdfs:Datatype>
                <owl:oneOf>
                    <rdf:Description>
                        <rdf:type rdf:resource="http://www.w3.org/1999/02/22-rdf-syntax-ns#List"/>
                        <rdf:first>Autumn</rdf:first>
                        <rdf:rest>
                            <rdf:Description>
                                <rdf:type rdf:resource="http://www.w3.org/1999/02/22-rdf-syntax-ns#List"/>
                                <rdf:first>Spring</rdf:first>
                                <rdf:rest>
                                    <rdf:Description>
                                        <rdf:type rdf:resource="http://www.w3.org/1999/02/22-rdf-syntax-ns#List"/>
                                        <rdf:first>Summer</rdf:first>
                                        <rdf:rest>
                                            <rdf:Description>
                                                <rdf:type rdf:resource="http://www.w3.org/1999/02/22-rdf-syntax-ns#List"/>
                                                <rdf:first>Winter</rdf:first>
                                                <rdf:rest rdf:resource="http://www.w3.org/1999/02/22-rdf-syntax-ns#nil"/>
                                            </rdf:Description>
                                        </rdf:rest>
                                    </rdf:Description>
                                </rdf:rest>
                            </rdf:Description>
                        </rdf:rest>
                    </rdf:Description>
                </owl:oneOf>
            </rdfs:Datatype>
        </rdfs:range>
        <rdfs:comment>It describes the season name associated to the date. It accepts
string values among “spring”, “summer”, “autumn”, “winter” and it is defined as a
generic RDF property</rdfs:comment>
    </owl:DatatypeProperty>
    


    <!-- http://seodwarf.eu/ontology/v1.0#hasSourceSatelliteName -->

    <owl:DatatypeProperty rdf:about="http://seodwarf.eu/ontology/v1.0#hasSourceSatelliteName">
        <rdf:type rdf:resource="http://www.w3.org/2002/07/owl#FunctionalProperty"/>
        <rdfs:domain rdf:resource="http://seodwarf.eu/ontology/v1.0#SatelliteImage"/>
        <rdfs:range>
            <rdfs:Datatype>
                <owl:oneOf>
                    <rdf:Description>
                        <rdf:type rdf:resource="http://www.w3.org/1999/02/22-rdf-syntax-ns#List"/>
                        <rdf:first>Sentinel 1</rdf:first>
                        <rdf:rest>
                            <rdf:Description>
                                <rdf:type rdf:resource="http://www.w3.org/1999/02/22-rdf-syntax-ns#List"/>
                                <rdf:first>Sentinel 2</rdf:first>
                                <rdf:rest>
                                    <rdf:Description>
                                        <rdf:type rdf:resource="http://www.w3.org/1999/02/22-rdf-syntax-ns#List"/>
                                        <rdf:first>Sentinel 3</rdf:first>
                                        <rdf:rest rdf:resource="http://www.w3.org/1999/02/22-rdf-syntax-ns#nil"/>
                                    </rdf:Description>
                                </rdf:rest>
                            </rdf:Description>
                        </rdf:rest>
                    </rdf:Description>
                </owl:oneOf>
            </rdfs:Datatype>
        </rdfs:range>
        <rdfs:comment>It describes the name of the satellite from which the
image came from. It accepts one of the following textual values: “Sentinel 1”,
“Sentinel 2”, “Sentinel 3”. It is defined as the “source” property of the Dublin Core
Ontology</rdfs:comment>
        <rdfs:isDefinedBy>dct:source</rdfs:isDefinedBy>
    </owl:DatatypeProperty>
    


    <!-- http://seodwarf.eu/ontology/v1.0#hasSouthLatitude -->

    <owl:DatatypeProperty rdf:about="http://seodwarf.eu/ontology/v1.0#hasSouthLatitude">
        <rdf:type rdf:resource="http://www.w3.org/2002/07/owl#FunctionalProperty"/>
        <rdfs:domain rdf:resource="http://seodwarf.eu/ontology/v1.0#BoxCoordinate"/>
        <rdfs:range rdf:resource="http://www.w3.org/2001/XMLSchema#float"/>
        <rdfs:comment>It describes the south latitude of the map box. It accepts
float values in the range -90 +90 that are less than the one of north latitude. It
is defined as a generic RDF property</rdfs:comment>
    </owl:DatatypeProperty>
    


    <!-- http://seodwarf.eu/ontology/v1.0#hasSpatialResolution -->

    <owl:DatatypeProperty rdf:about="http://seodwarf.eu/ontology/v1.0#hasSpatialResolution">
        <rdf:type rdf:resource="http://www.w3.org/2002/07/owl#FunctionalProperty"/>
        <rdfs:domain rdf:resource="http://seodwarf.eu/ontology/v1.0#SatelliteImage"/>
        <rdfs:range rdf:resource="http://www.w3.org/2001/XMLSchema#integer"/>
        <rdfs:comment>It describes the presence of a resolution value for the
image. It accepts numerical values and it is defined as a generic RDF property</rdfs:comment>
    </owl:DatatypeProperty>
    


    <!-- http://seodwarf.eu/ontology/v1.0#hasSpeedValue -->

    <owl:DatatypeProperty rdf:about="http://seodwarf.eu/ontology/v1.0#hasSpeedValue">
        <rdfs:domain rdf:resource="http://sweet.jpl.nasa.gov/2.3/propSpeed.owl#Speed"/>
        <rdfs:range rdf:resource="http://www.w3.org/2001/XMLSchema#float"/>
        <rdfs:comment>it refers to the value of the measurement of the speed. It accepts
floating point numbers as range.</rdfs:comment>
    </owl:DatatypeProperty>
    


    <!-- http://seodwarf.eu/ontology/v1.0#hasTemperatureValue -->

    <owl:DatatypeProperty rdf:about="http://seodwarf.eu/ontology/v1.0#hasTemperatureValue">
        <rdfs:domain rdf:resource="http://sweet.jpl.nasa.gov/2.3/propTemperature.owl#Temperature"/>
        <rdfs:range rdf:resource="http://www.w3.org/2001/XMLSchema#float"/>
        <rdfs:comment>It refers to the value of the measurement of the
temperature. It accepts floating point numbers as range</rdfs:comment>
    </owl:DatatypeProperty>
    


    <!-- http://seodwarf.eu/ontology/v1.0#hasTimestamp -->

    <owl:DatatypeProperty rdf:about="http://seodwarf.eu/ontology/v1.0#hasTimestamp">
        <rdfs:domain rdf:resource="http://sweet.jpl.nasa.gov/2.3/propTime.owl#Time"/>
        <rdfs:range rdf:resource="http://www.w3.org/2001/XMLSchema#long"/>
        <rdfs:comment>It describes the timestamp of acquisition of the image. It is
defined as the “temporal” property of the Dublin Core Ontology</rdfs:comment>
        <rdfs:isDefinedBy>dct:temporal</rdfs:isDefinedBy>
    </owl:DatatypeProperty>
    


    <!-- http://seodwarf.eu/ontology/v1.0#hasTitle -->

    <owl:DatatypeProperty rdf:about="http://seodwarf.eu/ontology/v1.0#hasTitle">
        <rdf:type rdf:resource="http://www.w3.org/2002/07/owl#FunctionalProperty"/>
        <rdfs:domain rdf:resource="http://seodwarf.eu/ontology/v1.0#SatelliteImage"/>
        <rdfs:range rdf:resource="http://www.w3.org/2001/XMLSchema#string"/>
        <rdfs:comment>It describes the title assigned to the image. It accepts alphanumerical
values and it is defined as the “title” property of the Dublin Core Ontology.</rdfs:comment>
        <rdfs:isDefinedBy>dct:title</rdfs:isDefinedBy>
    </owl:DatatypeProperty>
    


    <!-- http://seodwarf.eu/ontology/v1.0#hasTotalSuspendedSoilValue -->

    <owl:DatatypeProperty rdf:about="http://seodwarf.eu/ontology/v1.0#hasTotalSuspendedSoilValue">
        <rdfs:domain rdf:resource="http://sweet.jpl.nasa.gov/2.3/propChemical.owl#TotalSuspendedSolids"/>
        <rdfs:range rdf:resource="http://www.w3.org/2001/XMLSchema#float"/>
        <rdfs:comment>It refers to the quantity of solid particels in the
water. It accepts floating number values and is defined as a standard RDF property</rdfs:comment>
    </owl:DatatypeProperty>
    


    <!-- http://seodwarf.eu/ontology/v1.0#hasTurbidityValue -->

    <owl:DatatypeProperty rdf:about="http://seodwarf.eu/ontology/v1.0#hasTurbidityValue">
        <rdfs:domain rdf:resource="http://seodwarf.eu/ontology/v1.0#Turbidity"/>
        <rdfs:range rdf:resource="http://www.w3.org/2001/XMLSchema#float"/>
        <rdfs:comment>It refers to the numerical value of FTU assigned to the instance
of turbidity. It accepts floating numbers values and is defined as a standard RDF
property</rdfs:comment>
    </owl:DatatypeProperty>
    


    <!-- http://seodwarf.eu/ontology/v1.0#hasType -->

    <owl:DatatypeProperty rdf:about="http://seodwarf.eu/ontology/v1.0#hasType">
        <rdfs:domain rdf:resource="http://seodwarf.eu/ontology/v1.0#SatelliteImage"/>
        <rdfs:range rdf:resource="http://www.w3.org/2001/XMLSchema#string"/>
        <rdfs:comment>It describes the representation type of the image. It accepts
alphanumerical values</rdfs:comment>
    </owl:DatatypeProperty>
    


    <!-- http://seodwarf.eu/ontology/v1.0#hasURL -->

    <owl:DatatypeProperty rdf:about="http://seodwarf.eu/ontology/v1.0#hasURL">
        <rdf:type rdf:resource="http://www.w3.org/2002/07/owl#FunctionalProperty"/>
        <rdfs:domain rdf:resource="http://seodwarf.eu/ontology/v1.0#RegionType"/>
        <rdfs:range rdf:resource="http://www.w3.org/2001/XMLSchema#anyURI"/>
        <rdfs:comment>It describes the URL of the referring concept in GEMET. It accepts only
valid URLs. It is defined as the “source” property of the Dublin Core Ontology</rdfs:comment>
        <rdfs:isDefinedBy>dct:source</rdfs:isDefinedBy>
    </owl:DatatypeProperty>
    


    <!-- http://seodwarf.eu/ontology/v1.0#hasWestLongitude -->

    <owl:DatatypeProperty rdf:about="http://seodwarf.eu/ontology/v1.0#hasWestLongitude">
        <rdf:type rdf:resource="http://www.w3.org/2002/07/owl#FunctionalProperty"/>
        <rdfs:domain rdf:resource="http://seodwarf.eu/ontology/v1.0#BoxCoordinate"/>
        <rdfs:range rdf:resource="http://www.w3.org/2001/XMLSchema#float"/>
        <rdfs:comment>It describes the west longitude of the map box. It
accepts float values in the range -180 +180 that are less than the one of east
longitude. It is defined as a generic RDF property</rdfs:comment>
    </owl:DatatypeProperty>
    


    <!-- 
    ///////////////////////////////////////////////////////////////////////////////////////
    //
    // Classes
    //
    ///////////////////////////////////////////////////////////////////////////////////////
     -->

    


    <!-- http://seodwarf.eu/ontology/v1.0#Algae -->

    <owl:Class rdf:about="http://seodwarf.eu/ontology/v1.0#Algae">
        <owl:equivalentClass rdf:resource="http://sweet.jpl.nasa.gov/2.3/matrMicrobiota.owl#Algae"/>
        <rdfs:subClassOf rdf:resource="http://sweet.jpl.nasa.gov/2.3/matrPlant.owl#Plant"/>
        <rdfs:seeAlso>dbo:Algae</rdfs:seeAlso>
    </owl:Class>
    


    <!-- http://seodwarf.eu/ontology/v1.0#AlgalBloom -->

    <owl:Class rdf:about="http://seodwarf.eu/ontology/v1.0#AlgalBloom">
        <rdfs:subClassOf rdf:resource="http://seodwarf.eu/ontology/v1.0#OceanPhenomenon"/>
        <rdfs:comment>it refers to the rapid increase or accumulation in the population of algae in
a water system. The concept is placed as subclass of “seo:ocean_phenomenon” but it
is linked with the SWEET Ontology concept “algal bloom” and with the DBpedia concept
“Algal_Bloom”</rdfs:comment>
        <rdfs:seeAlso>dbo:Algal_Bloom</rdfs:seeAlso>
        <rdfs:seeAlso>swe:AlgalBloom</rdfs:seeAlso>
    </owl:Class>
    


    <!-- http://seodwarf.eu/ontology/v1.0#AverageTemperature -->

    <owl:Class rdf:about="http://seodwarf.eu/ontology/v1.0#AverageTemperature">
        <rdfs:subClassOf rdf:resource="http://sweet.jpl.nasa.gov/2.3/propTemperature.owl#Temperature"/>
        <rdfs:comment>The “seo:average_temperature” refers to the value of the average of the measurements of
the temperature in the area and acquires all the datatype properties of its parent</rdfs:comment>
    </owl:Class>
    


    <!-- http://seodwarf.eu/ontology/v1.0#BoxCoordinate -->

    <owl:Class rdf:about="http://seodwarf.eu/ontology/v1.0#BoxCoordinate">
        <rdfs:subClassOf rdf:resource="http://seodwarf.eu/ontology/v1.0#GeographicalCoordinate"/>
        <owl:disjointWith rdf:resource="http://seodwarf.eu/ontology/v1.0#PointCoordinate"/>
        <rdfs:comment>It identifies the coordinates used to define a box</rdfs:comment>
    </owl:Class>
    


    <!-- http://seodwarf.eu/ontology/v1.0#BrownAlgae -->

    <owl:Class rdf:about="http://seodwarf.eu/ontology/v1.0#BrownAlgae">
        <rdfs:subClassOf rdf:resource="http://seodwarf.eu/ontology/v1.0#Heteroknophyta"/>
    </owl:Class>
    


    <!-- http://seodwarf.eu/ontology/v1.0#CardinalDirection -->

    <owl:Class rdf:about="http://seodwarf.eu/ontology/v1.0#CardinalDirection">
        <rdfs:subClassOf rdf:resource="http://sweet.jpl.nasa.gov/2.3/reprDataModel.owl#Array"/>
        <rdfs:comment>The “seo:cardinal_direction” concept is defined as a subClassOf “swe:Array” and defines
in degrees the direction of the wind vector. North (N): 0° = 360°, East (E): 90°, South (S):
180°, West (W): 270°.</rdfs:comment>
        <rdfs:seeAlso>dbo:Cardinal_Direction</rdfs:seeAlso>
    </owl:Class>
    


    <!-- http://seodwarf.eu/ontology/v1.0#Chlorarachniophtya -->

    <owl:Class rdf:about="http://seodwarf.eu/ontology/v1.0#Chlorarachniophtya">
        <rdfs:subClassOf rdf:resource="http://seodwarf.eu/ontology/v1.0#Eukaryota"/>
    </owl:Class>
    


    <!-- http://seodwarf.eu/ontology/v1.0#ChlorophyllConcentration -->

    <owl:Class rdf:about="http://seodwarf.eu/ontology/v1.0#ChlorophyllConcentration">
        <rdfs:subClassOf rdf:resource="http://sweet.jpl.nasa.gov/2.3/propQuantity.owl#BiologicalQuantity"/>
        <rdfs:label>Chlo-a</rdfs:label>
    </owl:Class>
    


    <!-- http://seodwarf.eu/ontology/v1.0#Chlorophyta -->

    <owl:Class rdf:about="http://seodwarf.eu/ontology/v1.0#Chlorophyta">
        <rdfs:subClassOf rdf:resource="http://seodwarf.eu/ontology/v1.0#Eukaryota"/>
        <rdfs:comment>Green algae</rdfs:comment>
    </owl:Class>
    


    <!-- http://seodwarf.eu/ontology/v1.0#Cryptophyta -->

    <owl:Class rdf:about="http://seodwarf.eu/ontology/v1.0#Cryptophyta">
        <rdfs:subClassOf rdf:resource="http://seodwarf.eu/ontology/v1.0#Eukaryota"/>
        <rdfs:comment>Cryptomonads</rdfs:comment>
    </owl:Class>
    


    <!-- http://seodwarf.eu/ontology/v1.0#Cyanophyta -->

    <owl:Class rdf:about="http://seodwarf.eu/ontology/v1.0#Cyanophyta">
        <owl:equivalentClass rdf:resource="http://sweet.jpl.nasa.gov/2.3/matrMicrobiota.owl#BlueGreenAlgae"/>
        <rdfs:subClassOf rdf:resource="http://seodwarf.eu/ontology/v1.0#Prokaryota"/>
        <owl:disjointWith rdf:resource="http://seodwarf.eu/ontology/v1.0#Prochlorophyta"/>
        <rdfs:comment>Blue-green algae</rdfs:comment>
    </owl:Class>
    


    <!-- http://seodwarf.eu/ontology/v1.0#Diatoms -->

    <owl:Class rdf:about="http://seodwarf.eu/ontology/v1.0#Diatoms">
        <rdfs:subClassOf rdf:resource="http://seodwarf.eu/ontology/v1.0#Heteroknophyta"/>
    </owl:Class>
    


    <!-- http://seodwarf.eu/ontology/v1.0#Dinophyta -->

    <owl:Class rdf:about="http://seodwarf.eu/ontology/v1.0#Dinophyta">
        <rdfs:subClassOf rdf:resource="http://seodwarf.eu/ontology/v1.0#Eukaryota"/>
        <rdfs:comment>Dinoflagelates</rdfs:comment>
    </owl:Class>
    


    <!-- http://seodwarf.eu/ontology/v1.0#Euglenophyta -->

    <owl:Class rdf:about="http://seodwarf.eu/ontology/v1.0#Euglenophyta">
        <rdfs:subClassOf rdf:resource="http://seodwarf.eu/ontology/v1.0#Eukaryota"/>
        <rdfs:comment>Euglenoids</rdfs:comment>
    </owl:Class>
    


    <!-- http://seodwarf.eu/ontology/v1.0#Eukaryota -->

    <owl:Class rdf:about="http://seodwarf.eu/ontology/v1.0#Eukaryota">
        <rdfs:subClassOf rdf:resource="http://seodwarf.eu/ontology/v1.0#Algae"/>
        <owl:disjointWith rdf:resource="http://seodwarf.eu/ontology/v1.0#Prokaryota"/>
    </owl:Class>
    


    <!-- http://seodwarf.eu/ontology/v1.0#Front -->

    <owl:Class rdf:about="http://seodwarf.eu/ontology/v1.0#Front">
        <rdfs:subClassOf rdf:resource="http://seodwarf.eu/ontology/v1.0#OceanPhenomenon"/>
        <rdfs:comment>it refers to a boundary separating two water masses moving in two different
directions. The concept is placed as subclass of “seo:ocean_phenomenon” and it is
linked the DBpedia concept “Front_(oceanography)</rdfs:comment>
        <rdfs:seeAlso>dbo:Front(Oceanography)</rdfs:seeAlso>
    </owl:Class>
    


    <!-- http://seodwarf.eu/ontology/v1.0#GeographicalCoordinate -->

    <owl:Class rdf:about="http://seodwarf.eu/ontology/v1.0#GeographicalCoordinate">
        <rdfs:subClassOf rdf:resource="http://sweet.jpl.nasa.gov/2.3/repr.owl#CoordinateSystem"/>
        <rdfs:comment>The concept refers to the coordinate concept used to describe a point or a polygon in a geographical map. It has a reference to the DBpedia “Geographic_coordinate_system” concept for creating a linking point with the Linked
Open Data Cloud. The specific concept will be added as child of the “swe:Coordinate
System” concept</rdfs:comment>
        <rdfs:seeAlso>dbo:Dimension</rdfs:seeAlso>
    </owl:Class>
    


    <!-- http://seodwarf.eu/ontology/v1.0#Glaucophyta -->

    <owl:Class rdf:about="http://seodwarf.eu/ontology/v1.0#Glaucophyta">
        <rdfs:subClassOf rdf:resource="http://seodwarf.eu/ontology/v1.0#Eukaryota"/>
    </owl:Class>
    


    <!-- http://seodwarf.eu/ontology/v1.0#GoldenAlgae -->

    <owl:Class rdf:about="http://seodwarf.eu/ontology/v1.0#GoldenAlgae">
        <rdfs:subClassOf rdf:resource="http://seodwarf.eu/ontology/v1.0#Heteroknophyta"/>
    </owl:Class>
    


    <!-- http://seodwarf.eu/ontology/v1.0#Haptophyta -->

    <owl:Class rdf:about="http://seodwarf.eu/ontology/v1.0#Haptophyta">
        <rdfs:subClassOf rdf:resource="http://seodwarf.eu/ontology/v1.0#Eukaryota"/>
        <rdfs:comment>Coccolithophorids</rdfs:comment>
    </owl:Class>
    


    <!-- http://seodwarf.eu/ontology/v1.0#HarmfulAlgalBloom -->

    <owl:Class rdf:about="http://seodwarf.eu/ontology/v1.0#HarmfulAlgalBloom">
        <rdfs:subClassOf rdf:resource="http://seodwarf.eu/ontology/v1.0#AlgalBloom"/>
        <rdfs:comment>“Harmful Algal Bloom” is a specific type of Algal Bloom correlated with a
toxic species of algae</rdfs:comment>
    </owl:Class>
    


    <!-- http://seodwarf.eu/ontology/v1.0#Heteroknophyta -->

    <owl:Class rdf:about="http://seodwarf.eu/ontology/v1.0#Heteroknophyta">
        <rdfs:subClassOf rdf:resource="http://seodwarf.eu/ontology/v1.0#Eukaryota"/>
    </owl:Class>
    


    <!-- http://seodwarf.eu/ontology/v1.0#HotSpot -->

    <owl:Class rdf:about="http://seodwarf.eu/ontology/v1.0#HotSpot">
        <rdfs:subClassOf rdf:resource="http://seodwarf.eu/ontology/v1.0#OceanPhenomenon"/>
        <rdfs:comment>It is an area with higher water temperature than the temperatures recorded
usually</rdfs:comment>
    </owl:Class>
    


    <!-- http://seodwarf.eu/ontology/v1.0#Image -->

    <owl:Class rdf:about="http://seodwarf.eu/ontology/v1.0#Image">
        <rdfs:subClassOf rdf:resource="http://seodwarf.eu/ontology/v1.0#SatelliteImage"/>
        <rdfs:comment>The concept refers to a satellite image, used and archived in the project. It is the
source used for responding to the user queries. Searching in the SWEET Ontology, we
can identify the concept of “image” under the “Representation” class. The concept of
“image” is extended generating the class of “Satellite Image” and the class “seo:image”</rdfs:comment>
    </owl:Class>
    


    <!-- http://seodwarf.eu/ontology/v1.0#ImageContentArea -->

    <owl:Class rdf:about="http://seodwarf.eu/ontology/v1.0#ImageContentArea">
        <rdfs:subClassOf rdf:resource="http://sweet.jpl.nasa.gov/2.3/reprSpaceGeometry.owl#Region"/>
        <rdfs:comment>the concept refers to a specific region of the image that it is
relevant to describe it. The region has a name, a set of coordinates, a type, a geoname_id
if it is universally identified and a list of institutional area of reference (nations, regions,
province, cities). It refers to the DBpedia concept “Location_(geography)” for creating a
linking point with the Linked Open Data Cloud.</rdfs:comment>
    </owl:Class>
    


    <!-- http://seodwarf.eu/ontology/v1.0#LandSurfaceTemperature -->

    <owl:Class rdf:about="http://seodwarf.eu/ontology/v1.0#LandSurfaceTemperature">
        <rdfs:subClassOf rdf:resource="http://sweet.jpl.nasa.gov/2.3/propTemperature.owl#Temperature"/>
        <rdfs:comment>The “seo:land_surface_temperature” refers to the value of measurements of the temperature
over the land. It acquires all the datatype properties of its parent.</rdfs:comment>
        <rdfs:label>LST</rdfs:label>
    </owl:Class>
    


    <!-- http://seodwarf.eu/ontology/v1.0#MeanSeaLevel -->

    <owl:Class rdf:about="http://seodwarf.eu/ontology/v1.0#MeanSeaLevel">
        <rdfs:subClassOf rdf:resource="http://sweet.jpl.nasa.gov/2.3/propSpaceHeight.owl#SeaLevel"/>
        <rdfs:comment>The “seo:mean_sea_level” concept refers to the mean level of sea in the area</rdfs:comment>
    </owl:Class>
    


    <!-- http://seodwarf.eu/ontology/v1.0#MicrogramPerLiter -->

    <owl:Class rdf:about="http://seodwarf.eu/ontology/v1.0#MicrogramPerLiter">
        <rdfs:label>ug/L</rdfs:label>
    </owl:Class>
    


    <!-- http://seodwarf.eu/ontology/v1.0#MiligramPerLiter -->

    <owl:Class rdf:about="http://seodwarf.eu/ontology/v1.0#MiligramPerLiter">
        <rdfs:label>mg/L</rdfs:label>
    </owl:Class>
    


    <!-- http://seodwarf.eu/ontology/v1.0#OceanPhenomenon -->

    <owl:Class rdf:about="http://seodwarf.eu/ontology/v1.0#OceanPhenomenon">
        <owl:equivalentClass rdf:resource="http://sweet.jpl.nasa.gov/2.3/phenOcean.owl#OceanPhenomena"/>
        <rdfs:subClassOf rdf:resource="http://seodwarf.eu/ontology/v1.0#Phenomenon"/>
        <rdfs:seeAlso>swe:OceanPhenomena</rdfs:seeAlso>
    </owl:Class>
    


    <!-- http://seodwarf.eu/ontology/v1.0#OilSpill -->

    <owl:Class rdf:about="http://seodwarf.eu/ontology/v1.0#OilSpill">
        <owl:equivalentClass rdf:resource="http://sweet.jpl.nasa.gov/2.3/phenEnvirImpact.owl#OilSpill"/>
        <rdfs:subClassOf rdf:resource="http://seodwarf.eu/ontology/v1.0#OceanPhenomenon"/>
        <rdfs:comment>It refers to areas where liquid petroleum is released into the environment,
especially marine areas. The concept is placed as subclass of “seo:ocean_phenomenon”
but it is linked with the SWEET Ontology concept “oil spill” and with the DBpedia concept
“Oil_spill”</rdfs:comment>
        <rdfs:seeAlso>dbo:Oil_spill</rdfs:seeAlso>
        <rdfs:seeAlso>swe:Oil_Spill</rdfs:seeAlso>
    </owl:Class>
    


    <!-- http://seodwarf.eu/ontology/v1.0#Phenomenon -->

    <owl:Class rdf:about="http://seodwarf.eu/ontology/v1.0#Phenomenon">
        <owl:equivalentClass rdf:resource="http://sweet.jpl.nasa.gov/2.3/phen.owl#PlanetaryPhenomena"/>
        <rdfs:subClassOf rdf:resource="http://sweet.jpl.nasa.gov/2.3/phen.owl#Phenomena"/>
        <rdfs:comment>The general concept “phenomenon” is specialized into the
“ocean_phenomenon” and where possible, concepts and relations from other ontologies
are reused, while new concepts and relations are added if required. It refers to the
DBpedia concept “Phenomenon” for creating a linking point with the Linked Open Data
Cloud</rdfs:comment>
        <rdfs:seeAlso>swe:PlanetaryPhenomena</rdfs:seeAlso>
    </owl:Class>
    


    <!-- http://seodwarf.eu/ontology/v1.0#PointCoordinate -->

    <owl:Class rdf:about="http://seodwarf.eu/ontology/v1.0#PointCoordinate">
        <rdfs:subClassOf rdf:resource="http://seodwarf.eu/ontology/v1.0#GeographicalCoordinate"/>
        <rdfs:comment>It identifies the coordinates used to define a point</rdfs:comment>
    </owl:Class>
    


    <!-- http://seodwarf.eu/ontology/v1.0#Prochlorophyta -->

    <owl:Class rdf:about="http://seodwarf.eu/ontology/v1.0#Prochlorophyta">
        <rdfs:subClassOf rdf:resource="http://seodwarf.eu/ontology/v1.0#Prokaryota"/>
    </owl:Class>
    


    <!-- http://seodwarf.eu/ontology/v1.0#Prokaryota -->

    <owl:Class rdf:about="http://seodwarf.eu/ontology/v1.0#Prokaryota">
        <rdfs:subClassOf rdf:resource="http://seodwarf.eu/ontology/v1.0#Algae"/>
    </owl:Class>
    


    <!-- http://seodwarf.eu/ontology/v1.0#RegionType -->

    <owl:Class rdf:about="http://seodwarf.eu/ontology/v1.0#RegionType">
        <rdfs:subClassOf rdf:resource="http://sweet.jpl.nasa.gov/2.3/propCategorical.owl#Type"/>
        <rdfs:comment>the concept refers to a specific description able to geographically
characterize the region of interest. The concept is found in the SWEET Ontology as
“type”, but it is extended as following for creating a specific class to represent GEMET
Thesaurus types
The instances of the “region_type” class accepts as range the following elements:
 Natural Area or subclasses: https://www.eionet.europa.eu/gemet/concept?cp=5494&amp;langcode=en&amp;ns=1
 Built-up area or subclasses: https://www.eionet.europa.eu/gemet/concept?cp=1065&amp;langcode=en&amp;ns=1
 Sea or subclasses: https://www.eionet.europa.eu/gemet/concept?cp=7495&amp;langcode=en&amp;ns=1
 Lake or subclasses: https://www.eionet.europa.eu/gemet/concept?cp=4594&amp;langcode=en&amp;ns=1
 Watercourse or subclasses: https://www.eionet.europa.eu/gemet/concept?cp=9161&amp;langcode=en&amp;ns=1
 Water body or subclasses: https://www.eionet.europa.eu/gemet/concept?cp=9151&amp;langcode=en&amp;ns=1
 Water reservoir or subclasses: https://www.eionet.europa.eu/gemet/concept?cp=12248&amp;langcode=en&amp;ns=1</rdfs:comment>
    </owl:Class>
    


    <!-- http://seodwarf.eu/ontology/v1.0#Rhodophyta -->

    <owl:Class rdf:about="http://seodwarf.eu/ontology/v1.0#Rhodophyta">
        <rdfs:subClassOf rdf:resource="http://seodwarf.eu/ontology/v1.0#Eukaryota"/>
        <rdfs:comment>Red algae</rdfs:comment>
    </owl:Class>
    


    <!-- http://seodwarf.eu/ontology/v1.0#SSTAnomaly -->

    <owl:Class rdf:about="http://seodwarf.eu/ontology/v1.0#SSTAnomaly">
        <rdfs:subClassOf rdf:resource="http://seodwarf.eu/ontology/v1.0#SeaSurfaceTemperature"/>
        <rdfs:comment>the quantity of sst that is anomaly identified</rdfs:comment>
    </owl:Class>
    


    <!-- http://seodwarf.eu/ontology/v1.0#SSTNightime -->

    <owl:Class rdf:about="http://seodwarf.eu/ontology/v1.0#SSTNightime">
        <rdfs:subClassOf rdf:resource="http://seodwarf.eu/ontology/v1.0#SeaSurfaceTemperature"/>
        <rdfs:comment>sst in the night</rdfs:comment>
    </owl:Class>
    


    <!-- http://seodwarf.eu/ontology/v1.0#SatelliteImage -->

    <owl:Class rdf:about="http://seodwarf.eu/ontology/v1.0#SatelliteImage">
        <rdfs:subClassOf rdf:resource="http://sweet.jpl.nasa.gov/2.3/reprDataProduct.owl#Image"/>
        <rdfs:seeAlso>dbo:Satellite_imagery</rdfs:seeAlso>
    </owl:Class>
    


    <!-- http://seodwarf.eu/ontology/v1.0#SeaSurfaceTemperature -->

    <owl:Class rdf:about="http://seodwarf.eu/ontology/v1.0#SeaSurfaceTemperature">
        <rdfs:subClassOf rdf:resource="http://sweet.jpl.nasa.gov/2.3/propTemperature.owl#Temperature"/>
        <rdfs:comment>The “seo:sea_surface_temperature” refers to the value of measurements of the temperature
over the sea surface. It acquires all the datatype properties of its parent.</rdfs:comment>
        <rdfs:label>SST</rdfs:label>
    </owl:Class>
    


    <!-- http://seodwarf.eu/ontology/v1.0#ShallowWater -->

    <owl:Class rdf:about="http://seodwarf.eu/ontology/v1.0#ShallowWater">
        <rdfs:subClassOf rdf:resource="http://seodwarf.eu/ontology/v1.0#OceanPhenomenon"/>
        <rdfs:comment>it refers to phenomenon about the disruption of the natural orbital motion
of the wind. The concept is placed as subclass of “seo:ocean_phenomenon” and it is
linked the DBpedia concept “Waves_and_shallow_water”</rdfs:comment>
        <rdfs:seeAlso>dbo:Waves_and_Shallow_Water</rdfs:seeAlso>
    </owl:Class>
    


    <!-- http://seodwarf.eu/ontology/v1.0#TrophicStatusIndex -->

    <owl:Class rdf:about="http://seodwarf.eu/ontology/v1.0#TrophicStatusIndex">
        <rdfs:subClassOf rdf:resource="http://seodwarf.eu/ontology/v1.0#OceanPhenomenon"/>
        <rdfs:comment>It refers to the increase of nutrient concentrations followed by
corollary increases in subsequent trophic levels, such as eutrophication. The concept is
placed as subclass of “seo:ocean_phenomenon” and it is linked the DBpedia concept
“Trophic_state_index”</rdfs:comment>
        <rdfs:seeAlso>dbo:Trophic_state_index</rdfs:seeAlso>
    </owl:Class>
    


    <!-- http://seodwarf.eu/ontology/v1.0#Turbidity -->

    <owl:Class rdf:about="http://seodwarf.eu/ontology/v1.0#Turbidity">
        <owl:equivalentClass rdf:resource="http://sweet.jpl.nasa.gov/2.3/propIndex.owl#Turbidity"/>
        <rdfs:subClassOf rdf:resource="http://seodwarf.eu/ontology/v1.0#OceanPhenomenon"/>
        <rdfs:comment>it refers to the cloudiness or haziness of a fluid caused by large numbers of
individual particles. The concept is placed as subclass of “seo:ocean_phenomenon” but
it is linked with the SWEET Ontology concept “Turbidity” and with the DBpedia concept
“Turbidity”</rdfs:comment>
        <rdfs:seeAlso>dbo:Oil_Spill</rdfs:seeAlso>
        <rdfs:seeAlso>swe:OilSpill</rdfs:seeAlso>
    </owl:Class>
    


    <!-- http://seodwarf.eu/ontology/v1.0#Upwelling -->

    <owl:Class rdf:about="http://seodwarf.eu/ontology/v1.0#Upwelling">
        <rdfs:subClassOf rdf:resource="http://seodwarf.eu/ontology/v1.0#OceanPhenomenon"/>
        <rdfs:comment>It refers to areas where water with Sea Surface Temperature (SST) lower
than surrounding one is recorded. The concept is placed as subclass of
“seo:ocean_phenomenon” but it is linked with the SWEET Ontology concept “Upwelling”
and with the DBpedia concept “Upwelling”</rdfs:comment>
        <rdfs:seeAlso>dbo:Upwelling</rdfs:seeAlso>
        <rdfs:seeAlso>swe:Upwelling</rdfs:seeAlso>
    </owl:Class>
    


    <!-- http://seodwarf.eu/ontology/v1.0#Wave -->

    <owl:Class rdf:about="http://seodwarf.eu/ontology/v1.0#Wave">
        <rdfs:subClassOf rdf:resource="http://seodwarf.eu/ontology/v1.0#OceanPhenomenon"/>
        <rdfs:comment>it refers to the waves present on the sea surfaces. The concept is placed as
subclass of “seo:ocean_phenomenon” and it is linked the DBpedia concept
“Wind_wave”</rdfs:comment>
        <rdfs:seeAlso>dbo:Wind_Wave</rdfs:seeAlso>
    </owl:Class>
    


    <!-- http://seodwarf.eu/ontology/v1.0#Wind -->

    <owl:Class rdf:about="http://seodwarf.eu/ontology/v1.0#Wind">
        <owl:equivalentClass rdf:resource="http://sweet.jpl.nasa.gov/2.3/phenAtmoWindMesoscale.owl#OceanWind"/>
        <rdfs:subClassOf rdf:resource="http://seodwarf.eu/ontology/v1.0#OceanPhenomenon"/>
        <rdfs:comment>the concept refers to a sea surface wind that is a crucial parameter for operational
use and for studies in coastal regions. The concept is placed as subclass of
“seo:ocean_phenomenon” and it is linked with the SWEET Ontology concept “Ocean
Wind” and with the DBpedia concept “Wind”</rdfs:comment>
        <rdfs:seeAlso>dbo:Wind</rdfs:seeAlso>
        <rdfs:seeAlso>swe:OceanWind</rdfs:seeAlso>
    </owl:Class>
    


    <!-- http://seodwarf.eu/ontology/v1.0#YellowGreenAlgae -->

    <owl:Class rdf:about="http://seodwarf.eu/ontology/v1.0#YellowGreenAlgae">
        <rdfs:subClassOf rdf:resource="http://seodwarf.eu/ontology/v1.0#Heteroknophyta"/>
    </owl:Class>
    


    <!-- http://sweet.jpl.nasa.gov/2.3/matrMicrobiota.owl#Algae -->

    <rdf:Description rdf:about="http://sweet.jpl.nasa.gov/2.3/matrMicrobiota.owl#Algae"/>
    


    <!-- http://sweet.jpl.nasa.gov/2.3/matrMicrobiota.owl#BlueGreenAlgae -->

    <rdf:Description rdf:about="http://sweet.jpl.nasa.gov/2.3/matrMicrobiota.owl#BlueGreenAlgae"/>
    


    <!-- http://sweet.jpl.nasa.gov/2.3/phen.owl#PlanetaryPhenomena -->

    <rdf:Description rdf:about="http://sweet.jpl.nasa.gov/2.3/phen.owl#PlanetaryPhenomena"/>
    


    <!-- http://sweet.jpl.nasa.gov/2.3/phenAtmoWindMesoscale.owl#OceanWind -->

    <rdf:Description rdf:about="http://sweet.jpl.nasa.gov/2.3/phenAtmoWindMesoscale.owl#OceanWind"/>
    


    <!-- http://sweet.jpl.nasa.gov/2.3/phenEnvirImpact.owl#OilSpill -->

    <rdf:Description rdf:about="http://sweet.jpl.nasa.gov/2.3/phenEnvirImpact.owl#OilSpill"/>
    


    <!-- http://sweet.jpl.nasa.gov/2.3/phenOcean.owl#OceanPhenomena -->

    <rdf:Description rdf:about="http://sweet.jpl.nasa.gov/2.3/phenOcean.owl#OceanPhenomena"/>
    


    <!-- http://sweet.jpl.nasa.gov/2.3/propIndex.owl#Turbidity -->

    <rdf:Description rdf:about="http://sweet.jpl.nasa.gov/2.3/propIndex.owl#Turbidity"/>
    


    <!-- http://sweet.jpl.nasa.gov/2.3/propQuantity.owl#Quantity -->

    <rdf:Description rdf:about="http://sweet.jpl.nasa.gov/2.3/propQuantity.owl#Quantity">
        <rdfs:subClassOf rdf:resource="http://sweet.jpl.nasa.gov/2.3/propQuantity.owl#ScientificQuantity"/>
    </rdf:Description>
    


    <!-- 
    ///////////////////////////////////////////////////////////////////////////////////////
    //
    // General axioms
    //
    ///////////////////////////////////////////////////////////////////////////////////////
     -->

    <rdf:Description>
        <rdf:type rdf:resource="http://www.w3.org/2002/07/owl#AllDisjointClasses"/>
        <owl:members rdf:parseType="Collection">
            <rdf:Description rdf:about="http://seodwarf.eu/ontology/v1.0#AlgalBloom"/>
            <rdf:Description rdf:about="http://seodwarf.eu/ontology/v1.0#Front"/>
            <rdf:Description rdf:about="http://seodwarf.eu/ontology/v1.0#HotSpot"/>
            <rdf:Description rdf:about="http://seodwarf.eu/ontology/v1.0#OilSpill"/>
            <rdf:Description rdf:about="http://seodwarf.eu/ontology/v1.0#ShallowWater"/>
            <rdf:Description rdf:about="http://seodwarf.eu/ontology/v1.0#TrophicStatusIndex"/>
            <rdf:Description rdf:about="http://seodwarf.eu/ontology/v1.0#Turbidity"/>
            <rdf:Description rdf:about="http://seodwarf.eu/ontology/v1.0#Upwelling"/>
            <rdf:Description rdf:about="http://seodwarf.eu/ontology/v1.0#Wave"/>
            <rdf:Description rdf:about="http://seodwarf.eu/ontology/v1.0#Wind"/>
        </owl:members>
    </rdf:Description>
    <rdf:Description>
        <rdf:type rdf:resource="http://www.w3.org/2002/07/owl#AllDisjointClasses"/>
        <owl:members rdf:parseType="Collection">
            <rdf:Description rdf:about="http://seodwarf.eu/ontology/v1.0#BrownAlgae"/>
            <rdf:Description rdf:about="http://seodwarf.eu/ontology/v1.0#Diatoms"/>
            <rdf:Description rdf:about="http://seodwarf.eu/ontology/v1.0#GoldenAlgae"/>
            <rdf:Description rdf:about="http://seodwarf.eu/ontology/v1.0#YellowGreenAlgae"/>
        </owl:members>
    </rdf:Description>
    <rdf:Description>
        <rdf:type rdf:resource="http://www.w3.org/2002/07/owl#AllDisjointClasses"/>
        <owl:members rdf:parseType="Collection">
            <rdf:Description rdf:about="http://seodwarf.eu/ontology/v1.0#Chlorarachniophtya"/>
            <rdf:Description rdf:about="http://seodwarf.eu/ontology/v1.0#Chlorophyta"/>
            <rdf:Description rdf:about="http://seodwarf.eu/ontology/v1.0#Cryptophyta"/>
            <rdf:Description rdf:about="http://seodwarf.eu/ontology/v1.0#Dinophyta"/>
            <rdf:Description rdf:about="http://seodwarf.eu/ontology/v1.0#Euglenophyta"/>
            <rdf:Description rdf:about="http://seodwarf.eu/ontology/v1.0#Glaucophyta"/>
            <rdf:Description rdf:about="http://seodwarf.eu/ontology/v1.0#Haptophyta"/>
            <rdf:Description rdf:about="http://seodwarf.eu/ontology/v1.0#Heteroknophyta"/>
            <rdf:Description rdf:about="http://seodwarf.eu/ontology/v1.0#Rhodophyta"/>
        </owl:members>
    </rdf:Description>
</rdf:RDF>



<!-- Generated by the OWL API (version 4.2.6.20160910-2108) https://github.com/owlcs/owlapi -->

